Explicitly define the pad minimizer

runtime/proofs/mem.v
@@ -24,94 +24,102 @@ Proof.
       now rewrite <- N, <- M.
 Qed.
 
-Lemma pad_min a b c: a <> 0 -> c <> 0 ->
-  c mod a = 0 \/ a mod c = 0 ->
-  exists i, forall j, pad (a * i + b) c <= pad (a * j + b) c.
+Definition pad_minimizer a b c :=
+  if b mod c mod a =? 0
+  then c / a - b mod c / a
+  else c / a - 1 - b mod c / a.
+
+Lemma pad_min a b c: c mod a = 0 ->
+  let i := pad_minimizer a b c in
+  forall j, pad (a * i + b) c <= pad (a * j + b) c.
 Proof.
-  intros Anz Cnz.
-  destruct 1.
-  - destruct (proj1 (Nat.mod_divides _ a Anz) H) as [j J].
-    case (Nat.eq_dec (b mod c mod a) 0).
-    + intro R.
-      destruct (proj1 (Nat.mod_divides _ a Anz) R) as [k K].
-      exists (j - k).
-      intro i.
-      unfold pad.
-      rewrite <- (Nat.add_mod_idemp_r _ b c Cnz), K.
-      rewrite <- Nat.mul_add_distr_l.
-      assert (k <= j) as KJ. {
-        refine (Nat.lt_le_incl _ _ _).
-        pose (L := Nat.mod_upper_bound b c Cnz).
-        rewrite K, J in L.
-        exact (proj2 (Nat.mul_lt_mono_pos_l a k j (proj1 (Nat.neq_0_lt_0 _) Anz)) L).
-      }
-      rewrite (Nat.sub_add k j KJ).
-      rewrite <- J.
-      rewrite (Nat.mod_same _ Cnz).
-      apply Nat.le_0_l.
-    + intro R.
-      pose (k := b mod c / a).
-      pose (r := b mod c mod a).
+  intros CA m.
+  case (Nat.eq_dec c 0); [intro z; now rewrite z|]; intro Cnz.
+  case (Nat.eq_dec a 0); [intro z; now rewrite z|]; intro Anz.
+  destruct (proj1 (Nat.mod_divides _ a Anz) CA) as [j J].
+  case (Nat.eq_dec (b mod c mod a) 0).
+  + intros R i.
+    destruct (proj1 (Nat.mod_divides _ a Anz) R) as [k K].
 
-      destruct j; [exfalso; rewrite Nat.mul_0_r in J; now apply Cnz|].
-      exists (j - k).
-      intro i.
-      refine (pad_le Cnz _).
-      rewrite <- (Nat.add_mod_idemp_r _ b c Cnz).
-      rewrite <- (Nat.add_mod_idemp_r _ b c Cnz).
+    assert (m = j - k) as M. {
+      unfold m, pad_minimizer.
+      rewrite (proj2 (Nat.eqb_eq _ _) R), K, J.
+      now repeat rewrite Nat.mul_comm, (Nat.div_mul _ _ Anz).
+    }
+    rewrite M.
 
-      rewrite (Nat.div_mod (b mod c) a Anz).
-      fold k. fold r.
-
-      rewrite Nat.add_assoc, Nat.add_assoc.
-      rewrite <- Nat.mul_add_distr_l, <- Nat.mul_add_distr_l.
-
-      assert (k <= j) as KJ. {
-        unfold k.
-        refine (proj1 (Nat.lt_succ_r _ _) _).
-        refine (Nat.div_lt_upper_bound _ _ _ Anz _).
-        rewrite <- J.
-        exact (Nat.mod_upper_bound b c Cnz).
-      }
-      rewrite (Nat.sub_add _ _ KJ).
-
-      assert (a * j + r < c) as AJRC. {
-        rewrite J.
-        rewrite Nat.mul_succ_r.
-        refine (proj1 (Nat.add_lt_mono_l _ _ _) _).
-        apply (Nat.mod_upper_bound (b mod c) _ Anz).
-      }
-      rewrite (Nat.mod_small _ _ AJRC).
-
-      rewrite <- (Nat.add_mod_idemp_l _ _ c Cnz), J.
-      rewrite (Nat.mul_mod_distr_l _ _ _ (Nat.neq_succ_0 _) Anz).
-
-      assert (a * ((i + k) mod S j) + r < a * S j) as l. {
-        rewrite Nat.mul_succ_r.
-        refine (Nat.add_le_lt_mono _ _ _ _ _ _).
-        - refine (proj1 (Nat.mul_le_mono_pos_l _ _ _ (proj1 (Nat.neq_0_lt_0 _) Anz)) _).
-          refine (proj2 (Nat.succ_le_mono _ _) _).
-          exact (Nat.mod_upper_bound _ _ (Nat.neq_succ_0 _)).
-        - now apply Nat.mod_upper_bound.
-      }
-      rewrite (Nat.mod_small _ _ l).
-
-      split.
-      ++ rewrite <- (Nat.add_0_l 0).
-         refine (Nat.add_le_lt_mono _ _ _ _ (Nat.le_0_l _) _).
-         now refine (proj1 (Nat.neq_0_lt_0 _) _).
-      ++ refine (proj1 (Nat.add_le_mono_r _ _ _) _).
-         refine (proj1 (Nat.mul_le_mono_pos_l _ _ _ (proj1 (Nat.neq_0_lt_0 _) Anz)) _).
-         refine (proj1 (Nat.lt_succ_r _ _) _).
-         exact (Nat.mod_upper_bound _ _ (Nat.neq_succ_0 _)).
-  - destruct (proj1 (Nat.mod_divides _ _ Cnz) H) as [j J].
-    exists 0.
-    intro i.
     unfold pad.
-    rewrite J, Nat.mul_0_r, Nat.add_0_l.
-    rewrite <- (Nat.add_mod_idemp_l _ _ _ Cnz).
-    rewrite <- Nat.mul_assoc, Nat.mul_comm.
-    now rewrite (Nat.mod_mul _ _ Cnz), Nat.add_0_l.
+    rewrite <- (Nat.add_mod_idemp_r _ b c Cnz), K.
+    rewrite <- Nat.mul_add_distr_l.
+
+    assert (k <= j) as KJ. {
+      refine (Nat.lt_le_incl _ _ _).
+      pose (L := Nat.mod_upper_bound b c Cnz).
+      rewrite K, J in L.
+      exact (proj2 (Nat.mul_lt_mono_pos_l a k j (proj1 (Nat.neq_0_lt_0 _) Anz)) L).
+    }
+    rewrite (Nat.sub_add k j KJ).
+
+    rewrite <- J, (Nat.mod_same _ Cnz).
+    apply Nat.le_0_l.
+  + intros R i.
+    destruct j; [exfalso; rewrite Nat.mul_0_r in J; now apply Cnz|].
+
+    pose (k := b mod c / a).
+    pose (r := b mod c mod a).
+    assert (m = j - k) as M. {
+      unfold m, pad_minimizer.
+      rewrite (proj2 (Nat.eqb_neq _ _) R).
+      rewrite J.
+      rewrite Nat.mul_comm at 1.
+      now rewrite (Nat.div_mul _ _ Anz), Nat.sub_1_r, Nat.pred_succ, <- J.
+    }
+    rewrite M.
+
+    refine (pad_le Cnz _).
+    repeat rewrite <- (Nat.add_mod_idemp_r _ b c Cnz).
+    rewrite (Nat.div_mod (b mod c) a Anz).
+    fold k. fold r.
+    repeat rewrite Nat.add_assoc, <- Nat.mul_add_distr_l.
+
+    assert (k <= j) as KJ. {
+      unfold k.
+      refine (proj1 (Nat.lt_succ_r _ _) _).
+      refine (Nat.div_lt_upper_bound _ _ _ Anz _).
+      rewrite <- J.
+      exact (Nat.mod_upper_bound _ _ Cnz).
+    }
+    rewrite (Nat.sub_add _ _ KJ).
+
+    assert (a * j + r < c) as AJRC. {
+      rewrite J.
+      rewrite Nat.mul_succ_r.
+      refine (proj1 (Nat.add_lt_mono_l _ _ _) _).
+      apply (Nat.mod_upper_bound (b mod c) _ Anz).
+    }
+    rewrite (Nat.mod_small _ _ AJRC).
+
+    rewrite <- (Nat.add_mod_idemp_l _ _ _ Cnz), J.
+    rewrite (Nat.mul_mod_distr_l _ _ _ (Nat.neq_succ_0 _) Anz).
+
+    assert (a * ((i + k) mod S j) + r < a * S j) as l. {
+      rewrite Nat.mul_succ_r.
+      refine (Nat.add_le_lt_mono _ _ _ _ _ _).
+      - refine (proj1 (Nat.mul_le_mono_pos_l _ _ _ (proj1 (Nat.neq_0_lt_0 _) Anz)) _).
+        refine (proj2 (Nat.succ_le_mono _ _) _).
+        exact (Nat.mod_upper_bound _ _ (Nat.neq_succ_0 _)).
+      - now apply Nat.mod_upper_bound.
+    }
+    rewrite (Nat.mod_small _ _ l).
+
+    split.
+    ++ rewrite <- (Nat.add_0_l 0).
+       refine (Nat.add_le_lt_mono _ _ _ _ (Nat.le_0_l _) _).
+       now refine (proj1 (Nat.neq_0_lt_0 _) _).
+    ++ refine (proj1 (Nat.add_le_mono_r _ _ _) _).
+       refine (proj1 (Nat.mul_le_mono_pos_l _ _ _ (proj1 (Nat.neq_0_lt_0 _) Anz)) _).
+       refine (proj1 (Nat.lt_succ_r _ _) _).
+       exact (Nat.mod_upper_bound _ _ (Nat.neq_succ_0 _)).
 Qed.
 
 Definition aligned x N := N <> 0 /\ pad x N = 0.
